bitwise

src/Init/Data/SInt/Basic.lean
@@ -1626,7 +1626,7 @@ Convert an `ISize` to `BitVec 32`, assuming that the system bit-width is 32.
 This operation is intended for proof purposes.
 -/
 def ISize.toBitVec32 (a : ISize) (h : System.Platform.numBits = 32) : BitVec 32 :=
-  h ▸ a.toBitVec
+  a.toBitVec.cast h
 
 /--
 Convert an `ISize` to `BitVec 64`, assuming that the system bit-width is 64.
@@ -1634,7 +1634,7 @@ Convert an `ISize` to `BitVec 64`, assuming that the system bit-width is 64.
 This operation is intended for proof purposes.
 -/
 def ISize.toBitVec64 (a : ISize) (h : System.Platform.numBits = 64) : BitVec 64 :=
-  h ▸ a.toBitVec
+  a.toBitVec.cast h
 
 /-- Obtains the `ISize` that is 2's complement equivalent to the `USize`. -/
 @[inline] def USize.toISize (i : USize) : ISize := ISize.ofUSize i
