src/Init/Data/UInt/Basic.lean
@@ -940,15 +940,15 @@ Convert a `USize` to `BitVec 32`, assuming that the system bit-width is 32.
 This operation is intended for proof purposes.
 -/
 def USize.toBitVec32 (a : USize) (h : System.Platform.numBits = 32) : BitVec 32 :=
-  h ▸ a.toBitVec
+  a.toBitVec.cast h
 
 /--
-Convert a `USize` to `BitVec 64`, assuming that the system bit-width is 32.
+Convert a `USize` to `BitVec 64`, assuming that the system bit-width is 64.
 
 This operation is intended for proof purposes.
 -/
 def USize.toBitVec64 (a : USize) (h : System.Platform.numBits = 64) : BitVec 64 :=
-  h ▸ a.toBitVec
+  a.toBitVec.cast h
 
 instance : Mul USize       := ⟨USize.mul⟩
 instance : Pow USize Nat   := ⟨USize.pow⟩
