tests/elab/int_toBitVec.lean
@@ -10,8 +10,8 @@ example (a b c d e : UInt32) : ((a + (b * c)) = (b - d / e)) ↔ (a.toBitVec + b
 example (a b c d e : UInt64) : ((a + (b * c)) = (b - d / e)) ↔ (a.toBitVec + b.toBitVec * c.toBitVec = b.toBitVec - d.toBitVec / e.toBitVec) := by
   simp only [int_toBitVec]
 
-example (a b c d e : USize) : ((a + (b * c)) = (b - d / e)) ↔ (a.toBitVec + b.toBitVec * c.toBitVec = b.toBitVec - d.toBitVec / e.toBitVec) := by
-  simp only [int_toBitVec]
+example (a b c d e : USize) (h : System.Platform.numBits = 64) : ((a + (b * c)) = (b - d / e)) ↔ (a.toBitVec64 h + b.toBitVec64 h * c.toBitVec64 h = b.toBitVec64 h - d.toBitVec64 h / e.toBitVec64 h) := by
+  simp only [int_toBitVec, h]
 
 example (a b c d e : UInt8) : ((a + (b * c)) < (b - d / e)) ↔ (a.toBitVec + b.toBitVec * c.toBitVec < b.toBitVec - d.toBitVec / e.toBitVec) := by
   simp only [int_toBitVec]
@@ -25,8 +25,8 @@ example (a b c d e : UInt32) : ((a + (b * c)) < (b - d / e)) ↔ (a.toBitVec + b
 example (a b c d e : UInt64) : ((a + (b * c)) < (b - d / e)) ↔ (a.toBitVec + b.toBitVec * c.toBitVec < b.toBitVec - d.toBitVec / e.toBitVec) := by
   simp only [int_toBitVec]
 
-example (a b c d e : USize) : ((a + (b * c)) < (b - d / e)) ↔ (a.toBitVec + b.toBitVec * c.toBitVec < b.toBitVec - d.toBitVec / e.toBitVec) := by
-  simp only [int_toBitVec]
+example (a b c d e : USize) (h : System.Platform.numBits = 64) : ((a + (b * c)) < (b - d / e)) ↔ (a.toBitVec64 h + b.toBitVec64 h * c.toBitVec64 h < b.toBitVec64 h - d.toBitVec64 h / e.toBitVec64 h) := by
+  simp only [int_toBitVec, h]
 
 example (a b c d e : UInt8) : ((a + (b * c)) ≤ (b - d / e)) ↔ (a.toBitVec + b.toBitVec * c.toBitVec ≤ b.toBitVec - d.toBitVec / e.toBitVec) := by
   simp only [int_toBitVec]
@@ -40,5 +40,5 @@ example (a b c d e : UInt32) : ((a + (b * c)) ≤ (b - d / e)) ↔ (a.toBitVec +
 example (a b c d e : UInt64) : ((a + (b * c)) ≤ (b - d / e)) ↔ (a.toBitVec + b.toBitVec * c.toBitVec ≤ b.toBitVec - d.toBitVec / e.toBitVec) := by
   simp only [int_toBitVec]
 
-example (a b c d e : USize) : ((a + (b * c)) ≤ (b - d / e)) ↔ (a.toBitVec + b.toBitVec * c.toBitVec ≤ b.toBitVec - d.toBitVec / e.toBitVec) := by
-  simp only [int_toBitVec]
+example (a b c d e : USize) (h : System.Platform.numBits = 64) : ((a + (b * c)) ≤ (b - d / e)) ↔ (a.toBitVec64 h + b.toBitVec64 h * c.toBitVec64 h ≤ b.toBitVec64 h - d.toBitVec64 h / e.toBitVec64 h) := by
+  simp only [int_toBitVec, h]
